DynamoDbEncryption/runtimes/net/Generated/DynamoDbEncryption/TypeConversion.cs
@@ -1357,21 +1357,21 @@ namespace AWS.Cryptography.DbEncryptionSDK.DynamoDb
     {
       switch (value)
       {
-        case software.amazon.cryptography.dbencryptionsdk.dynamodb.internaldafny.types.Error_AwsCryptographyMaterialProviders dafnyVal:
-          return AWS.Cryptography.MaterialProviders.TypeConversion.FromDafny_CommonError(
-            dafnyVal._AwsCryptographyMaterialProviders
-          );
-        case software.amazon.cryptography.dbencryptionsdk.dynamodb.internaldafny.types.Error_AwsCryptographyPrimitives dafnyVal:
-          return AWS.Cryptography.Primitives.TypeConversion.FromDafny_CommonError(
-            dafnyVal._AwsCryptographyPrimitives
-          );
         case software.amazon.cryptography.dbencryptionsdk.dynamodb.internaldafny.types.Error_AwsCryptographyDbEncryptionSdkStructuredEncryption dafnyVal:
           return AWS.Cryptography.DbEncryptionSDK.StructuredEncryption.TypeConversion.FromDafny_CommonError(
             dafnyVal._AwsCryptographyDbEncryptionSdkStructuredEncryption
           );
+        case software.amazon.cryptography.dbencryptionsdk.dynamodb.internaldafny.types.Error_AwsCryptographyMaterialProviders dafnyVal:
+          return AWS.Cryptography.MaterialProviders.TypeConversion.FromDafny_CommonError(
+            dafnyVal._AwsCryptographyMaterialProviders
+          );
         case software.amazon.cryptography.dbencryptionsdk.dynamodb.internaldafny.types.Error_ComAmazonawsDynamodb dafnyVal:
           return Com.Amazonaws.Dynamodb.TypeConversion.FromDafny_CommonError(
             dafnyVal._ComAmazonawsDynamodb
+          );
+        case software.amazon.cryptography.dbencryptionsdk.dynamodb.internaldafny.types.Error_AwsCryptographyPrimitives dafnyVal:
+          return AWS.Cryptography.Primitives.TypeConversion.FromDafny_CommonError(
+            dafnyVal._AwsCryptographyPrimitives
           );
         case software.amazon.cryptography.dbencryptionsdk.dynamodb.internaldafny.types.Error_DynamoDbEncryptionException dafnyVal:
           return FromDafny_N3_aws__N12_cryptography__N15_dbEncryptionSdk__N8_dynamoDb__S27_DynamoDbEncryptionException(dafnyVal);
