DynamoDbEncryption/runtimes/net/Generated/DynamoDbEncryptionTransforms/TypeConversion.cs
@@ -4567,6 +4567,7 @@ namespace AWS.Cryptography.DbEncryptionSDK.DynamoDb.Transforms
     public static AWS.Cryptography.DbEncryptionSDK.StructuredEncryption.CryptoAction FromDafny_N3_aws__N12_cryptography__N15_dbEncryptionSdk__N20_structuredEncryption__S12_CryptoAction(software.amazon.cryptography.dbencryptionsdk.structuredencryption.internaldafny.types._ICryptoAction value)
     {
       if (value.is_ENCRYPT__AND__SIGN) return AWS.Cryptography.DbEncryptionSDK.StructuredEncryption.CryptoAction.ENCRYPT_AND_SIGN;
+      if (value.is_CONTEXT__AND__SIGN) return AWS.Cryptography.DbEncryptionSDK.StructuredEncryption.CryptoAction.CONTEXT_AND_SIGN;
       if (value.is_SIGN__ONLY) return AWS.Cryptography.DbEncryptionSDK.StructuredEncryption.CryptoAction.SIGN_ONLY;
       if (value.is_DO__NOTHING) return AWS.Cryptography.DbEncryptionSDK.StructuredEncryption.CryptoAction.DO_NOTHING;
       throw new System.ArgumentException("Invalid AWS.Cryptography.DbEncryptionSDK.StructuredEncryption.CryptoAction value");
@@ -4574,6 +4575,7 @@ namespace AWS.Cryptography.DbEncryptionSDK.DynamoDb.Transforms
     public static software.amazon.cryptography.dbencryptionsdk.structuredencryption.internaldafny.types._ICryptoAction ToDafny_N3_aws__N12_cryptography__N15_dbEncryptionSdk__N20_structuredEncryption__S12_CryptoAction(AWS.Cryptography.DbEncryptionSDK.StructuredEncryption.CryptoAction value)
     {
       if (AWS.Cryptography.DbEncryptionSDK.StructuredEncryption.CryptoAction.ENCRYPT_AND_SIGN.Equals(value)) return software.amazon.cryptography.dbencryptionsdk.structuredencryption.internaldafny.types.CryptoAction.create_ENCRYPT__AND__SIGN();
+      if (AWS.Cryptography.DbEncryptionSDK.StructuredEncryption.CryptoAction.CONTEXT_AND_SIGN.Equals(value)) return software.amazon.cryptography.dbencryptionsdk.structuredencryption.internaldafny.types.CryptoAction.create_CONTEXT__AND__SIGN();
       if (AWS.Cryptography.DbEncryptionSDK.StructuredEncryption.CryptoAction.SIGN_ONLY.Equals(value)) return software.amazon.cryptography.dbencryptionsdk.structuredencryption.internaldafny.types.CryptoAction.create_SIGN__ONLY();
       if (AWS.Cryptography.DbEncryptionSDK.StructuredEncryption.CryptoAction.DO_NOTHING.Equals(value)) return software.amazon.cryptography.dbencryptionsdk.structuredencryption.internaldafny.types.CryptoAction.create_DO__NOTHING();
       throw new System.ArgumentException("Invalid AWS.Cryptography.DbEncryptionSDK.StructuredEncryption.CryptoAction value");
@@ -6483,9 +6485,9 @@ namespace AWS.Cryptography.DbEncryptionSDK.DynamoDb.Transforms
     {
       switch (value)
       {
-        case software.amazon.cryptography.dbencryptionsdk.dynamodb.transforms.internaldafny.types.Error_AwsCryptographyDbEncryptionSdkDynamoDb dafnyVal:
-          return AWS.Cryptography.DbEncryptionSDK.DynamoDb.TypeConversion.FromDafny_CommonError(
-            dafnyVal._AwsCryptographyDbEncryptionSdkDynamoDb
+        case software.amazon.cryptography.dbencryptionsdk.dynamodb.transforms.internaldafny.types.Error_AwsCryptographyDbEncryptionSdkDynamoDbItemEncryptor dafnyVal:
+          return AWS.Cryptography.DbEncryptionSDK.DynamoDb.ItemEncryptor.TypeConversion.FromDafny_CommonError(
+            dafnyVal._AwsCryptographyDbEncryptionSdkDynamoDbItemEncryptor
           );
         case software.amazon.cryptography.dbencryptionsdk.dynamodb.transforms.internaldafny.types.Error_AwsCryptographyMaterialProviders dafnyVal:
           return AWS.Cryptography.MaterialProviders.TypeConversion.FromDafny_CommonError(
@@ -6495,13 +6497,13 @@ namespace AWS.Cryptography.DbEncryptionSDK.DynamoDb.Transforms
           return Com.Amazonaws.Dynamodb.TypeConversion.FromDafny_CommonError(
             dafnyVal._ComAmazonawsDynamodb
           );
+        case software.amazon.cryptography.dbencryptionsdk.dynamodb.transforms.internaldafny.types.Error_AwsCryptographyDbEncryptionSdkDynamoDb dafnyVal:
+          return AWS.Cryptography.DbEncryptionSDK.DynamoDb.TypeConversion.FromDafny_CommonError(
+            dafnyVal._AwsCryptographyDbEncryptionSdkDynamoDb
+          );
         case software.amazon.cryptography.dbencryptionsdk.dynamodb.transforms.internaldafny.types.Error_AwsCryptographyDbEncryptionSdkStructuredEncryption dafnyVal:
           return AWS.Cryptography.DbEncryptionSDK.StructuredEncryption.TypeConversion.FromDafny_CommonError(
             dafnyVal._AwsCryptographyDbEncryptionSdkStructuredEncryption
-          );
-        case software.amazon.cryptography.dbencryptionsdk.dynamodb.transforms.internaldafny.types.Error_AwsCryptographyDbEncryptionSdkDynamoDbItemEncryptor dafnyVal:
-          return AWS.Cryptography.DbEncryptionSDK.DynamoDb.ItemEncryptor.TypeConversion.FromDafny_CommonError(
-            dafnyVal._AwsCryptographyDbEncryptionSdkDynamoDbItemEncryptor
           );
         case software.amazon.cryptography.dbencryptionsdk.dynamodb.transforms.internaldafny.types.Error_DynamoDbEncryptionTransformsException dafnyVal:
           return FromDafny_N3_aws__N12_cryptography__N15_dbEncryptionSdk__N8_dynamoDb__N10_transforms__S37_DynamoDbEncryptionTransformsException(dafnyVal);
