DynamoDbEncryption/runtimes/net/Generated/StructuredEncryption/CryptoAction.cs
@@ -12,11 +12,13 @@ namespace AWS.Cryptography.DbEncryptionSDK.StructuredEncryption
 
     public static readonly CryptoAction ENCRYPT_AND_SIGN = new CryptoAction("ENCRYPT_AND_SIGN");
 
+    public static readonly CryptoAction CONTEXT_AND_SIGN = new CryptoAction("CONTEXT_AND_SIGN");
+
     public static readonly CryptoAction SIGN_ONLY = new CryptoAction("SIGN_ONLY");
 
     public static readonly CryptoAction DO_NOTHING = new CryptoAction("DO_NOTHING");
     public static readonly CryptoAction[] Values =  {
- DO_NOTHING , ENCRYPT_AND_SIGN , SIGN_ONLY
+ CONTEXT_AND_SIGN , DO_NOTHING , ENCRYPT_AND_SIGN , SIGN_ONLY
 };
     public CryptoAction(string value) : base(value) { }
   }
