DynamoDbEncryption/dafny/DynamoDbEncryptionTransforms/Model/AwsCryptographyDbEncryptionSdkDynamoDbTransformsTypes.dfy
@@ -740,7 +740,7 @@ include "../../../../submodules/MaterialProviders/StandardLibrary/src/Index.dfy"
  import Operations : AbstractAwsCryptographyDbEncryptionSdkDynamoDbTransformsOperations
  function method DefaultDynamoDbTablesEncryptionConfig(): AwsCryptographyDbEncryptionSdkDynamoDbTypes.DynamoDbTablesEncryptionConfig
  method DynamoDbEncryptionTransforms(config: AwsCryptographyDbEncryptionSdkDynamoDbTypes.DynamoDbTablesEncryptionConfig := DefaultDynamoDbTablesEncryptionConfig())
- returns (res: Result<DynamoDbEncryptionTransformsClient, Error>)
+ returns (res: Result<IDynamoDbEncryptionTransformsClient, Error>)
 // BEGIN MANUAL EDIT
  requires var tmps0 := set t0 | t0 in config.tableEncryptionConfigs.Values;
  forall tmp0 :: tmp0 in tmps0 ==>
